retrieve WIP

theories/lang/lang.v
@@ -443,6 +443,18 @@ Definition copy_from_addr_to_addr_unsafe (st : state) (src dst : Addr) (l : Word
 Definition copy_page_segment_unsafe (st : state) (src dst : PID) (l : Word) : state :=
   copy_from_addr_to_addr_unsafe st (of_pid src) (of_pid dst) l.
 
+Definition write_retrieve_msg (st:state) (dst: Addr) (wh:handle) (trn: transaction): option state:=
+ match trn with
+  | (vs, f, _ ,vr, ls, t) =>
+    match finz.of_z (Z.of_nat (length ls)) with
+    | Some l =>
+      Some (write_mem_segment_unsafe st dst
+                                      ([of_imm (encode_vmid vs); f; wh; encode_transaction_type t ;l;
+                                       of_imm (encode_vmid vr)] ++ map of_pid ls))
+    | None => None
+    end
+ end.
+
 Definition fill_rx_unsafe (st : state) (l : Word) (v r : VMID) (tx rx : PID) : state :=
   (get_reg_files st, vinsert r (tx, (rx, Some(l, v))) (get_mail_boxes st), get_page_tables st, get_current_vm st, get_mem st, get_transactions st).
 
@@ -700,8 +712,7 @@ Definition retrieve (s : state) : exec_mode * state :=
         trn <- lift_option_with_err (get_transaction s handle) InvParam ;;;
         (let (r, ps) := get_memory_descriptor trn in
          let ty := get_transaction_type trn in
-         (* add receiver(caller) into the list of the transaction *)
-         s' <- transfer_msg s len (get_current_vm s) ;;;
+         s' <- lift_option_with_err (write_retrieve_msg s (get_rx_pid_global s (get_current_vm s)) handle trn) InvParam ;;;
          (* for all pages of the trancation ... (change the page table of the caller according to the type)*)
          match ty with
          | Sharing =>
